\documentclass[11pt,fleqn,a4paper]{article}

\usepackage[a4paper,bottom=0cm]{geometry}
\usepackage{url}
\usepackage{amsmath}
\setlength{\voffset}{-0.75in}
\setlength{\headsep}{5pt}

\newcommand{\half}{\frac{1}{2}}
\newcommand{\mainEquation}{\( \sum\limits_{i=0}^{n} k^i = \frac{k ^{n + 1} - 1}{k - 1} \quad 0 \leq n < \infty  \)}

\begin{document}
\title{Proof that \mainEquation}
\date{}
\maketitle

\[ \sum\limits_{i=0}^{n} k^i = \frac{k ^{n + 1} - 1}{k - 1} \]

\[(k - 1)  \sum\limits_{i=0}^{n} k^i = k ^{n + 1} - 1\]

\[\sum\limits_{i=0}^{n} (k - 1) k^i = k ^{n + 1} - 1\]

\[\sum\limits_{i=0}^{n} (k^{i + 1} - k^i) = k ^{n + 1} - 1\]

\[\sum\limits_{i=0}^{n} k^{i + 1} - \sum\limits_{i=0}^{n} k^i = k ^{n + 1} - 1\]

\[\sum\limits_{i=1}^{n + 1} k^{i} - \sum\limits_{i=0}^{n} k^i = k ^{n + 1} - 1\]

\[\sum\limits_{i=n + 1}^{n + 1} k^{i} + \sum\limits_{i=1}^{n} k^{i} - \sum\limits_{i=0}^{0} k^i  - \sum\limits_{i=1}^{n} k^i = k ^{n + 1} - 1\]

\[\sum\limits_{i=n + 1}^{n + 1} k^{i} - \sum\limits_{i=0}^{0} k^i = k ^{n + 1} - 1\]

\[k ^{n + 1} - 1 = k ^{n + 1} - 1\]

\end{document}