\documentclass[11pt,fleqn,a4paper,leqno]{article}

\usepackage[a4paper,bottom=0cm]{geometry}
\usepackage{url}
\usepackage{amsmath}
\setlength{\voffset}{-0.75in}
\setlength{\headsep}{5pt}

\begin{document}
\title{Proof that \( \binom{n}{m} + \binom{n}{m + 1} = \binom{n + 1}{m + 1} \) }
\date{}
\maketitle

\[ \text{Find identities for each term} \]
\begin{equation}
\binom{n}{m} = \frac{n!}{m!(n - m)!} 
\end{equation}
\begin{equation}
\binom{n}{m + 1} = \frac{n!}{(m + 1)!(n - (m + 1))!}
\end{equation}
  
\[ (m+1)! = (m + 1)m! \]
\[ (n - (m + 1))! = (n - m - 1)! = \frac{(n - m)!}{n - m} \]

\begin{equation}
\binom{n}{m + 1} = \frac{n!}{(m + 1)m!\left[\frac{(n - m)!}{n -m }\right]}
\end{equation}
\begin{equation}
\binom{n}{m + 1} = \frac{n!}{\left[\frac{(m + 1)}{n -m }\right]m!(n - m)!}
\end{equation}
\begin{equation}
\binom{n + 1}{m + 1} = \frac{(n + 1)!}{(m+1)!((n + 1) - (m + 1))!}
\end{equation}
\begin{equation}
\binom{n + 1}{m + 1} = \frac{(n + 1)n!}{(m + 1)m!(n - m)!}
\end{equation}

\[ \text{Substitute in our new identities } \]
\[ \binom{n}{m} + \binom{n}{m + 1} = \binom{n + 1}{m + 1} \]
\begin{equation}
\frac{n!}{m!(n - m)!} + \frac{n!}{\left[\frac{(m + 1)}{n -m }\right]m!(n - m)!} = 
\frac{(n + 1)n!}{(m + 1)m!(n - m)!}
\end{equation}

\[ \text{Prove the equality } \]
\[ \text{Divide by \quad} \frac{n!}{m!(n - m)!} \]
\begin{equation}
1 + \frac{1}{\left[\frac{m + 1}{n - m}\right]} = \frac{n + 1}{m + 1}
\end{equation}

\[ \text{Multiply by \quad} m + 1 \]
\begin{equation}
m +1 + n -m = n + 1
\end{equation}

\end{document}